code/ed25519/Hacl.Impl.Ed25519.Sign.Steps.fst
@@ -5,13 +5,18 @@ open FStar.HyperStack.All
 open FStar.Mul
 
 open Lib.IntTypes
-open Lib.ByteSequence
-open Lib.Sequence
 open Lib.Buffer
 
+module BSeq = Lib.ByteSequence
+module LSeq = Lib.Sequence
+
 module F51 = Hacl.Impl.Ed25519.Field51
-module F56 = Hacl.Impl.BignumQ.Mul
-module S56 = Hacl.Spec.BignumQ.Definitions
+module BQ = Hacl.Impl.BignumQ
+
+module BD = Hacl.Bignum.Definitions
+module BN = Hacl.Bignum
+module SD = Hacl.Spec.Bignum.Definitions
+module SN = Hacl.Spec.Bignum
 
 #set-options "--z3rlimit 10 --max_fuel 0 --max_ifuel 0"
 
@@ -38,95 +43,56 @@ let point_mul_g_compress out s =
 
 
 inline_for_extraction noextract
-val sign_step_1:
-    secret:lbuffer uint8 32ul
-  -> tmp_bytes:lbuffer uint8 352ul ->
-  Stack unit
-    (requires fun h ->
-      live h secret /\ live h tmp_bytes /\ disjoint secret tmp_bytes)
-    (ensures fun h0 _ h1 -> modifies (loc tmp_bytes) h0 h1 /\
-      (let a, prefix = Spec.Ed25519.secret_expand (as_seq h0 secret) in
-        as_seq h1 (gsub tmp_bytes 224ul 32ul) == a /\
-        as_seq h1 (gsub tmp_bytes 256ul 32ul) == prefix /\
-        as_seq h1 (gsub tmp_bytes 96ul 32ul) ==
-        Spec.Ed25519.point_compress (Spec.Ed25519.point_mul a Spec.Ed25519.g)))
-
-let sign_step_1 secret tmp_bytes =
-  let a''    = sub tmp_bytes 96ul  32ul in
-  let apre   = sub tmp_bytes 224ul 64ul in
-  let a      = sub apre 0ul 32ul in
-  let prefix = sub apre 32ul 32ul in
-  Hacl.Impl.Ed25519.SecretExpand.secret_expand apre secret;
-  point_mul_g_compress a'' a
-
-
-inline_for_extraction noextract
 val sign_step_2:
     len:size_t{v len + 64 <= max_size_t}
   -> msg:lbuffer uint8 len
-  -> tmp_bytes:lbuffer uint8 352ul
-  -> tmp_ints:lbuffer uint64 65ul ->
+  -> tmp_bytes:lbuffer uint8 192ul
+  -> tmp_ints:lbuffer uint64 16ul ->
   Stack unit
     (requires fun h ->
       live h msg /\ live h tmp_bytes /\ live h tmp_ints /\
       disjoint tmp_bytes msg /\ disjoint tmp_bytes tmp_ints /\
       disjoint tmp_ints msg)
     (ensures fun h0 _ h1 -> modifies (loc tmp_ints) h0 h1 /\
-    (let s = as_seq h1 (gsub tmp_ints 20ul 5ul) in
-       v (Seq.index s 0) < pow2 56 /\
-       v (Seq.index s 1) < pow2 56 /\
-       v (Seq.index s 2) < pow2 56 /\
-       v (Seq.index s 3) < pow2 56 /\
-       v (Seq.index s 4) < pow2 32) /\
-      F56.as_nat h1 (gsub tmp_ints 20ul 5ul) == Spec.Ed25519.sha512_modq (32 + v len)
-        (concat #uint8 #32 #(v len) (as_seq h0 (gsub tmp_bytes 256ul 32ul)) (as_seq h0 msg)))
+      BD.bn_v h1 (gsub tmp_ints 0ul 4ul) == Spec.Ed25519.sha512_modq (32 + v len)
+        (LSeq.concat #uint8 #32 #(v len) (as_seq h0 (gsub tmp_bytes 160ul 32ul)) (as_seq h0 msg)))
 
 let sign_step_2 len msg tmp_bytes tmp_ints =
-  let r      = sub tmp_ints 20ul 5ul  in
-  let a''    = sub tmp_bytes 96ul  32ul in
-  let apre   = sub tmp_bytes 224ul 64ul in
-  let a      = sub apre 0ul 32ul in
-  let prefix = sub apre 32ul 32ul in
+  let r      = sub tmp_ints 0ul 4ul  in
+  let prefix = sub tmp_bytes 160ul 32ul in
   Hacl.Impl.SHA512.ModQ.sha512_modq_pre r prefix len msg
 
 
 inline_for_extraction noextract
 val sign_step_3:
-    tmp_bytes:lbuffer uint8 352ul
-  -> tmp_ints:lbuffer uint64 65ul ->
+    tmp_bytes:lbuffer uint8 192ul
+  -> tmp_ints:lbuffer uint64 16ul ->
   Stack unit
     (requires fun h ->
-      live h tmp_bytes /\ live h tmp_ints /\ disjoint tmp_bytes tmp_ints /\
-      (let s = as_seq h (gsub tmp_ints 20ul 5ul) in
-       v (Seq.index s 0) < pow2 56 /\
-       v (Seq.index s 1) < pow2 56 /\
-       v (Seq.index s 2) < pow2 56 /\
-       v (Seq.index s 3) < pow2 56 /\
-       v (Seq.index s 4) < pow2 32)
-    )
+      live h tmp_bytes /\ live h tmp_ints /\ disjoint tmp_bytes tmp_ints)
     (ensures fun h0 _ h1 -> modifies (loc tmp_bytes) h0 h1 /\
       // Framing
-      as_seq h0 (gsub tmp_bytes 96ul 32ul) == as_seq h1 (gsub tmp_bytes 96ul 32ul) /\
-      as_seq h0 (gsub tmp_bytes 224ul 32ul) == as_seq h1 (gsub tmp_bytes 224ul 32ul) /\
+      as_seq h0 (gsub tmp_bytes 0ul 32ul) == as_seq h1 (gsub tmp_bytes 0ul 32ul) /\
+      as_seq h0 (gsub tmp_bytes 128ul 32ul) == as_seq h1 (gsub tmp_bytes 128ul 32ul) /\
       // Postcondition
-      (assert_norm (pow2 56 < pow2 64); assert_norm (pow2 32 < pow2 64);
-        assert_norm (S56.as_nat5 (u64 (pow2 56 - 1), u64 (pow2 56 - 1), u64 (pow2 56 - 1), u64 (pow2 56 - 1), u64 (pow2 32 - 1)) < pow2 256);
-      as_seq h1 (gsub tmp_bytes 160ul 32ul) ==
+     (SD.bn_eval_bound (as_seq h0 (gsub tmp_ints 0ul 4ul)) 4;
+      as_seq h1 (gsub tmp_bytes 64ul 32ul) ==
       Spec.Ed25519.point_compress (Spec.Ed25519.point_mul
-        (nat_to_bytes_le 32 (F56.as_nat h0 (gsub tmp_ints 20ul 5ul)))
-        (Spec.Ed25519.g))))
+        (BSeq.nat_to_bytes_le 32 (BD.bn_v h0 (gsub tmp_ints 0ul 4ul))) Spec.Ed25519.g)))
 
 let sign_step_3 tmp_bytes tmp_ints =
-  let a''  = sub tmp_bytes 96ul  32ul in
-  let apre = sub tmp_bytes 224ul 64ul in
+  let a''  = sub tmp_bytes 0ul  32ul in
+  let apre = sub tmp_bytes 128ul 64ul in
   let a    = sub apre 0ul 32ul in
   push_frame();
   let rb = create 32ul (u8 0) in
-  let r  = sub tmp_ints 20ul 5ul  in
-  let rs' = sub tmp_bytes 160ul 32ul in
+  let r  = sub tmp_ints 0ul 4ul  in
+  let rs' = sub tmp_bytes 64ul 32ul in
+
   let h0 = ST.get() in
-  Hacl.Impl.Store56.store_56 rb r;
-  let h1 = ST.get() in
+  BN.bn_to_bytes_le 32ul r rb;
+  SD.bn_eval_bound (as_seq h0 r) 4;
+  SN.bn_to_bytes_le_lemma 32 (as_seq h0 r);
   point_mul_g_compress rs' rb;
   pop_frame()
 
@@ -135,8 +101,8 @@ inline_for_extraction noextract
 val sign_step_4:
     len:size_t{v len + 64 <= max_size_t}
   -> msg:lbuffer uint8 len
-  -> tmp_bytes:lbuffer uint8 352ul
-  -> tmp_ints:lbuffer uint64 65ul ->
+  -> tmp_bytes:lbuffer uint8 192ul
+  -> tmp_ints:lbuffer uint64 16ul ->
   Stack unit
     (requires fun h ->
       live h msg /\ live h tmp_bytes /\ live h tmp_ints /\
@@ -144,67 +110,61 @@ val sign_step_4:
       disjoint tmp_ints msg)
     (ensures fun h0 _ h1 -> modifies (loc tmp_ints) h0 h1 /\
       // Framing
-      as_seq h0 (gsub tmp_ints 20ul 5ul) == as_seq h1 (gsub tmp_ints 20ul 5ul) /\
+      as_seq h0 (gsub tmp_ints 0ul 4ul) == as_seq h1 (gsub tmp_ints 0ul 4ul) /\
       // Postcondition
-      F56.qelem_fits h1 (gsub tmp_ints 60ul 5ul) (1, 1, 1, 1, 1) /\
-      F56.as_nat h1 (gsub tmp_ints 60ul 5ul) ==
+      BD.bn_v h1 (gsub tmp_ints 12ul 4ul) ==
       Spec.Ed25519.sha512_modq (64 + v len)
-        (concat #uint8 #64 #(v len)
-          (concat #uint8 #32 #32
-            (as_seq h0 (gsub tmp_bytes 160ul 32ul))
-            (as_seq h0 (gsub tmp_bytes 96ul 32ul)))
+        (LSeq.concat #uint8 #64 #(v len)
+          (LSeq.concat #uint8 #32 #32
+            (as_seq h0 (gsub tmp_bytes 64ul 32ul))
+            (as_seq h0 (gsub tmp_bytes 0ul 32ul)))
           (as_seq h0 msg)
         )
       )
 
 let sign_step_4 len msg tmp_bytes tmp_ints =
-  let tmp_bytes' = tmp_bytes in
-  let r    = sub tmp_ints 20ul 5ul  in
-  let h    = sub tmp_ints 60ul 5ul  in
-  let a''  = sub tmp_bytes 96ul  32ul in
-  let rb   = sub tmp_bytes 128ul 32ul in
-  let rs'  = sub tmp_bytes 160ul 32ul in
-  let apre = sub tmp_bytes 224ul 64ul in
-  let a    = sub apre 0ul 32ul in
-  assert_norm (pow2 56 == 0x100000000000000);
+  let r    = sub tmp_ints 0ul 4ul  in
+  let h    = sub tmp_ints 12ul 4ul  in
+  let a''  = sub tmp_bytes 0ul  32ul in
+  let rs'  = sub tmp_bytes 64ul 32ul in
   Hacl.Impl.SHA512.ModQ.sha512_modq_pre_pre2 h rs' a'' len msg
 
 
 inline_for_extraction noextract
 val sign_step_5:
-    tmp_bytes:lbuffer uint8 352ul
-  -> tmp_ints:lbuffer uint64 65ul ->
+    tmp_bytes:lbuffer uint8 192ul
+  -> tmp_ints:lbuffer uint64 16ul ->
   Stack unit
     (requires fun h ->
       live h tmp_bytes /\ live h tmp_ints /\ disjoint tmp_bytes tmp_ints /\
-      F56.qelem_fits h (gsub tmp_ints 60ul 5ul) (1, 1, 1, 1, 1) /\
-      F56.qelem_fits h (gsub tmp_ints 20ul 5ul) (1, 1, 1, 1, 1) /\
-      F56.as_nat h (gsub tmp_ints 20ul 5ul) < Spec.Ed25519.q /\
-      F56.as_nat h (gsub tmp_ints 60ul 5ul) < pow2 256
+      BD.bn_v h (gsub tmp_ints 0ul 4ul) < Spec.Ed25519.q /\
+      BD.bn_v h (gsub tmp_ints 12ul 4ul) < Spec.Ed25519.q
     )
     (ensures fun h0 _ h1 -> modifies (loc tmp_bytes |+| loc tmp_ints) h0 h1 /\
       // Framing
-      as_seq h0 (gsub tmp_bytes 160ul 32ul) == as_seq h1 (gsub tmp_bytes 160ul 32ul) /\
+      as_seq h0 (gsub tmp_bytes 64ul 32ul) == as_seq h1 (gsub tmp_bytes 64ul 32ul) /\
       // Postcondition
-      (let r = F56.as_nat h0 (gsub tmp_ints 20ul 5ul) in
-       let h = F56.as_nat h0 (gsub tmp_ints 60ul 5ul) in
-       let a = as_seq h0 (gsub tmp_bytes 224ul 32ul) in
-      nat_from_bytes_le (as_seq h1 (gsub tmp_bytes 192ul 32ul)) ==
-      (r + (h * nat_from_bytes_le a) % Spec.Ed25519.q) % Spec.Ed25519.q))
+      (let r = BD.bn_v h0 (gsub tmp_ints 0ul 4ul) in
+       let h = BD.bn_v h0 (gsub tmp_ints 12ul 4ul) in
+       let a = as_seq h0 (gsub tmp_bytes 128ul 32ul) in
+      BSeq.nat_from_bytes_le (as_seq h1 (gsub tmp_bytes 96ul 32ul)) ==
+      (r + h * BSeq.nat_from_bytes_le a) % Spec.Ed25519.q))
 
 #set-options "--z3rlimit 40"
 
 let sign_step_5 tmp_bytes tmp_ints =
-  let r    = sub tmp_ints 20ul 5ul  in
-  let aq   = sub tmp_ints 45ul 5ul  in
-  let ha   = sub tmp_ints 50ul 5ul  in
-  let s    = sub tmp_ints 55ul 5ul  in
-  let h    = sub tmp_ints 60ul 5ul  in
-  let s'   = sub tmp_bytes 192ul 32ul in
-  let rs'  = sub tmp_bytes 160ul 32ul in
-  let a = sub tmp_bytes 224ul 32ul in
-  Hacl.Impl.Load56.load_32_bytes aq a;
-  Hacl.Impl.BignumQ.Mul.mul_modq ha h aq;
-  Hacl.Impl.BignumQ.Mul.add_modq s r ha;
-  assert_norm (0x100000000000000 == pow2 56);
-  Hacl.Impl.Store56.store_56 s' s
+  let r    = sub tmp_ints 0ul 4ul  in
+  let aq   = sub tmp_ints 4ul 4ul  in
+  let s    = sub tmp_ints 8ul 4ul  in
+  let h    = sub tmp_ints 12ul 4ul  in
+
+  let s'   = sub tmp_bytes 96ul 32ul in
+  let rs'  = sub tmp_bytes 64ul 32ul in
+  let a    = sub tmp_bytes 128ul 32ul in
+  let h0 = ST.get () in
+  BN.bn_from_bytes_le 32ul a aq;
+  SN.bn_from_bytes_le_lemma #U64 32 (as_seq h0 a);
+  BQ.mul_add_modq h aq r s;
+  let h1 = ST.get () in
+  BN.bn_to_bytes_le 32ul s s';
+  SN.bn_to_bytes_le_lemma 32 (as_seq h1 s)
