code/ed25519/Hacl.Impl.Ed25519.Verify.fst
@@ -5,13 +5,20 @@ open FStar.HyperStack.All
 open FStar.Mul
 
 open Lib.IntTypes
-open Lib.Sequence
-open Lib.ByteSequence
 open Lib.Buffer
 
 open Hacl.Bignum25519
 
+module LSeq = Lib.Sequence
+module BSeq = Lib.ByteSequence
+
 module F51 = Hacl.Impl.Ed25519.Field51
+module BQ = Hacl.Impl.BignumQ
+
+module BD = Hacl.Bignum.Definitions
+module BN = Hacl.Bignum
+module SD = Hacl.Spec.Bignum.Definitions
+module SB = Hacl.Spec.Bignum
 
 #reset-options "--z3rlimit 20 --max_fuel 0 --max_ifuel 0"
 
@@ -27,10 +34,10 @@ val verify_step_1:
       live h r /\ live h msg /\ live h rs /\ live h public /\
       disjoint msg r /\ disjoint rs r /\ disjoint public r)
     (ensures fun h0 _ h1 -> modifies (loc r) h0 h1 /\
-     as_seq h1 r == nat_to_bytes_le 32 (
+     as_seq h1 r == BSeq.nat_to_bytes_le 32 (
       Spec.Ed25519.sha512_modq (64 + v len)
-        (concat #uint8 #64 #(v len)
-          (concat #uint8 #32 #32
+        (LSeq.concat #uint8 #64 #(v len)
+          (LSeq.concat #uint8 #32 #32
             (as_seq h0 rs)
             (as_seq h0 public))
           (as_seq h0 msg)
@@ -38,10 +45,13 @@ val verify_step_1:
     )
 let verify_step_1 r msg len rs public =
   push_frame();
-  let r' = create 5ul (u64 0) in
+  let r' = create 4ul (u64 0) in
   Hacl.Impl.SHA512.ModQ.sha512_modq_pre_pre2 r' rs public msg len;
-  Hacl.Impl.Store56.store_56 r r';
+  let h0 = ST.get () in
+  BN.bn_to_bytes_le 32ul r' r;
+  SB.bn_to_bytes_le_lemma 32 (as_seq h0 r');
   pop_frame()
+
 
 inline_for_extraction noextract
 val verify_step_2':
@@ -99,13 +109,14 @@ let verify_step_2 s h' a' r' =
   pop_frame();
   b
 
+
 inline_for_extraction noextract
-val verify_inner_:
+val verify_step_3:
     public:lbuffer uint8 32ul
   -> len:size_t{v len + 64 <= max_size_t}
   -> msg:lbuffer uint8 len
   -> signature:lbuffer uint8 64ul
-  -> tmp:lbuffer uint64 45ul
+  -> tmp:lbuffer uint64 44ul
   -> tmp':lbuffer uint8 32ul ->
   Stack bool
     (requires fun h ->
@@ -124,28 +135,29 @@ val verify_inner_:
 
 #push-options "--z3rlimit 200"
 
-let verify_inner_ public len msg signature tmp tmp' =
+let verify_step_3 public len msg signature tmp tmp' =
   let rs = sub signature 0ul 32ul in
   let a' = sub tmp 0ul  20ul in
   let r' = sub tmp 20ul 20ul in
-  let s  = sub tmp 40ul 5ul  in
+  let s  = sub tmp 40ul 4ul  in
   (**) let h0 = get() in
-  Hacl.Impl.Load56.load_32_bytes s (sub signature 32ul 32ul);
+  BN.bn_from_bytes_le 32ul (sub signature 32ul 32ul) s;
+  SB.bn_from_bytes_le_lemma #U64 32 (as_seq h0 (gsub signature 32ul 32ul));
   let b'' = Hacl.Impl.Ed25519.PointEqual.gte_q s in
   if b'' then false
   else (
     verify_step_1 tmp' len msg rs public;
-    (**) lemma_nat_from_to_bytes_le_preserves_value (slice #uint8 #64 (as_seq h0 signature) 32 64) 32;
+    (**) BSeq.lemma_nat_from_to_bytes_le_preserves_value (LSeq.slice #uint8 #64 (as_seq h0 signature) 32 64) 32;
     verify_step_2 (sub signature 32ul 32ul) tmp' a' r')
 
 
 inline_for_extraction noextract
-val verify_:
+val verify_step_4:
     public:lbuffer uint8 32ul
   -> len:size_t{v len + 64 <= max_size_t}
   -> msg:lbuffer uint8 len
   -> signature:lbuffer uint8 64ul
-  -> tmp:lbuffer uint64 45ul
+  -> tmp:lbuffer uint64 44ul
   -> tmp':lbuffer uint8 32ul ->
   Stack bool
     (requires fun h ->
@@ -158,10 +170,10 @@ val verify_:
       z == Spec.Ed25519.verify (as_seq h0 public) (as_seq h0 msg) (as_seq h0 signature)
     )
 
-let verify_ public msg len signature tmp tmp' =
+let verify_step_4 public msg len signature tmp tmp' =
   let a' = sub tmp 0ul  20ul in
   let r' = sub tmp 20ul 20ul in
-  let s  = sub tmp 40ul 5ul  in
+  let s  = sub tmp 40ul 4ul  in
   let h'  = tmp' in
   let b = Hacl.Impl.Ed25519.PointDecompress.point_decompress a' public in
   let res =
@@ -169,7 +181,7 @@ let verify_ public msg len signature tmp tmp' =
     let rs = sub signature 0ul 32ul in
     let b' = Hacl.Impl.Ed25519.PointDecompress.point_decompress r' rs in
     if b' then (
-      verify_inner_ public msg len signature tmp tmp'
+      verify_step_3 public msg len signature tmp tmp'
     ) else false
   ) else false in
   res
@@ -191,8 +203,8 @@ val verify:
     )
 let verify public msg len signature =
   push_frame();
-  let tmp = create 45ul (u64 0) in
+  let tmp = create 44ul (u64 0) in
   let tmp' = create 32ul (u8 0) in
-  let res = verify_ public msg len signature tmp tmp' in
+  let res = verify_step_4 public msg len signature tmp tmp' in
   pop_frame();
   res
