code/ed25519/Hacl.Impl.SHA512.ModQ.fst
@@ -4,11 +4,15 @@ module ST = FStar.HyperStack.ST
 open FStar.HyperStack.All
 
 open Lib.IntTypes
-open Lib.ByteSequence
-open Lib.Sequence
 open Lib.Buffer
 
-module F56 = Hacl.Impl.BignumQ.Mul
+module LSeq = Lib.Sequence
+module BSeq = Lib.ByteSequence
+
+module BQ = Hacl.Impl.BignumQ
+module BD = Hacl.Bignum.Definitions
+module BN = Hacl.Bignum
+module SN = Hacl.Spec.Bignum
 
 #reset-options "--z3rlimit 200 --max_fuel 0 --max_ifuel 0"
 
@@ -24,7 +28,7 @@ val sha512_pre_msg:
       disjoint input hash /\ disjoint prefix hash)
     (ensures fun h0 _ h1 -> modifies (loc hash) h0 h1 /\
       as_seq h1 hash == Spec.Agile.Hash.hash Spec.Hash.Definitions.SHA2_512
-           (concat #uint8 #32 #(v len) (as_seq h0 prefix) (as_seq h0 input))
+           (LSeq.concat #uint8 #32 #(v len) (as_seq h0 prefix) (as_seq h0 input))
     )
 
 [@CInline]
@@ -51,8 +55,8 @@ val sha512_pre_pre2_msg:
     )
     (ensures fun h0 _ h1 -> modifies (loc hash) h0 h1 /\
       as_seq h1 hash == Spec.Agile.Hash.hash Spec.Hash.Definitions.SHA2_512
-        (concat #uint8 #64 #(v len)
-          (concat #uint8 #32 #32 (as_seq h0 prefix) (as_seq h0 prefix2))
+        (LSeq.concat #uint8 #64 #(v len)
+          (LSeq.concat #uint8 #32 #32 (as_seq h0 prefix) (as_seq h0 prefix2))
           (as_seq h0 input)
         )
     )
@@ -68,7 +72,7 @@ let sha512_pre_pre2_msg h prefix prefix2 len input =
 
 
 val sha512_modq_pre:
-    out:lbuffer uint64 5ul
+    out:lbuffer uint64 4ul
   -> prefix:lbuffer uint8 32ul
   -> len:size_t{v len + 32 <= max_size_t}
   -> input:lbuffer uint8 len ->
@@ -77,31 +81,25 @@ val sha512_modq_pre:
       live h input /\ live h out /\ live h prefix /\
       disjoint prefix out /\  disjoint out input)
     (ensures  fun h0 _ h1 -> modifies (loc out) h0 h1 /\
-      (let s = as_seq h1 out in
-       v (Seq.index s 0) < pow2 56 /\
-       v (Seq.index s 1) < pow2 56 /\
-       v (Seq.index s 2) < pow2 56 /\
-       v (Seq.index s 3) < pow2 56 /\
-       v (Seq.index s 4) < pow2 32) /\
-      F56.as_nat h1 out ==
+      BD.bn_v h1 out ==
       Spec.Ed25519.sha512_modq (32 + v len)
-        (concat #uint8 #32 #(v len) (as_seq h0 prefix) (as_seq h0 input))
-    )
+        (LSeq.concat #uint8 #32 #(v len) (as_seq h0 prefix) (as_seq h0 input)))
 
 [@CInline]
 let sha512_modq_pre out prefix len input =
   push_frame();
-  let tmp = create 10ul (u64 0) in
+  let tmp = create 8ul (u64 0) in
   let hash = create 64ul (u8 0) in
   sha512_pre_msg hash prefix len input;
-  Hacl.Impl.Load56.load_64_bytes tmp hash;
-  Hacl.Impl.BignumQ.Mul.barrett_reduction out tmp;
-  assert_norm (pow2 56 == 0x100000000000000);
+  let h0 = ST.get () in
+  BN.bn_from_bytes_le 64ul hash tmp;
+  SN.bn_from_bytes_le_lemma #U64 64 (as_seq h0 hash);
+  BQ.modq tmp out;
   pop_frame()
 
 
 val sha512_modq_pre_pre2:
-    out:lbuffer uint64 5ul
+    out:lbuffer uint64 4ul
   -> prefix:lbuffer uint8 32ul
   -> prefix2:lbuffer uint8 32ul
   -> len:size_t{v len + 64 <= max_size_t}
@@ -111,16 +109,10 @@ val sha512_modq_pre_pre2:
       live h input /\ live h out /\ live h prefix /\ live h prefix2 /\
       disjoint prefix out /\ disjoint prefix2 out /\ disjoint out input)
     (ensures  fun h0 _ h1 ->  modifies (loc out) h0 h1 /\
-      (let s = as_seq h1 out in
-       v (Seq.index s 0) < pow2 56 /\
-       v (Seq.index s 1) < pow2 56 /\
-       v (Seq.index s 2) < pow2 56 /\
-       v (Seq.index s 3) < pow2 56 /\
-       v (Seq.index s 4) < pow2 32) /\
-     F56.as_nat h1 out ==
+      BD.bn_v h1 out ==
       Spec.Ed25519.sha512_modq (64 + v len)
-        (concat #uint8 #64 #(v len)
-          (concat #uint8 #32 #32
+        (LSeq.concat #uint8 #64 #(v len)
+          (LSeq.concat #uint8 #32 #32
             (as_seq h0 prefix)
             (as_seq h0 prefix2))
           (as_seq h0 input)
@@ -130,10 +122,11 @@ val sha512_modq_pre_pre2:
 [@CInline]
 let sha512_modq_pre_pre2 out prefix prefix2 len input =
   push_frame();
-  let tmp = create 10ul (u64 0) in
+  let tmp = create 8ul (u64 0) in
   let hash = create 64ul (u8 0) in
   sha512_pre_pre2_msg hash prefix prefix2 len input;
-  Hacl.Impl.Load56.load_64_bytes tmp hash;
-  Hacl.Impl.BignumQ.Mul.barrett_reduction out tmp;
-  assert_norm (pow2 56 == 0x100000000000000);
+  let h0 = ST.get () in
+  BN.bn_from_bytes_le 64ul hash tmp;
+  SN.bn_from_bytes_le_lemma #U64 64 (as_seq h0 hash);
+  BQ.modq tmp out;
   pop_frame()
