code/ed25519/Hacl.Impl.BignumQ.fst
@@ -1,0 +1,142 @@
+module Hacl.Impl.BignumQ
+
+module ST = FStar.HyperStack.ST
+open FStar.HyperStack
+open FStar.HyperStack.All
+open FStar.Mul
+
+open Lib.IntTypes
+open Lib.Buffer
+
+module BD = Hacl.Bignum.Definitions
+module BN = Hacl.Bignum
+module BM = Hacl.Bignum.Montgomery
+module AM = Hacl.Bignum.AlmostMontgomery
+module BR = Hacl.Bignum.ModReduction
+
+module SD = Hacl.Spec.Bignum.Definitions
+module SN = Hacl.Spec.Bignum
+module SM = Hacl.Spec.Bignum.Montgomery
+
+#reset-options "--z3rlimit 50 --fuel 0 --ifuel 0"
+
+val lemma_mul_lt: a:nat -> b:nat -> c:nat -> d:nat -> Lemma
+  (requires a < c /\ b < d)
+  (ensures  a * b < c * d)
+let lemma_mul_lt a b c d = ()
+
+
+val make_q: q:lbuffer uint64 4ul ->
+  Stack unit
+  (requires fun h -> live h q)
+  (ensures  fun h0 _ h1 -> modifies (loc q) h0 h1 /\
+    BD.bn_v h1 q == Spec.Ed25519.q)
+
+[@CInline]
+let make_q q =
+  q.(0ul) <- u64 0x5812631a5cf5d3ed;
+  q.(1ul) <- u64 0x14def9dea2f79cd6;
+  q.(2ul) <- u64 0x0;
+  q.(3ul) <- u64 0x1000000000000000;
+  assert_norm (Spec.Ed25519.q == 0x5812631a5cf5d3ed + 0x14def9dea2f79cd6 * pow2 64 + 0x1000000000000000 * pow2 192);
+  let h = ST.get () in
+  SD.bn_eval_unfold_i (as_seq h q) 4;
+  SD.bn_eval_unfold_i (as_seq h q) 3;
+  SD.bn_eval_unfold_i (as_seq h q) 2;
+  SD.bn_eval_unfold_i (as_seq h q) 1;
+  SD.bn_eval0 (as_seq h q)
+
+
+inline_for_extraction noextract
+val make_mu: unit ->
+  Stack uint64
+  (requires fun h -> True)
+  (ensures  fun h0 mu h1 -> modifies0 h0 h1 /\
+    (1 + Spec.Ed25519.q * v mu) % pow2 64 == 0)
+
+let make_mu () =
+  let mu = u64 0xd2b51da312547e1b in
+  assert_norm ((1 + Spec.Ed25519.q * v mu) % pow2 64 = 0);
+  mu
+
+
+val make_r2_modq: r2:lbuffer uint64 4ul ->
+  Stack unit
+  (requires fun h -> live h r2)
+  (ensures  fun h0 _ h1 -> modifies (loc r2) h0 h1 /\
+    BD.bn_v h1 r2 == pow2 512 % Spec.Ed25519.q)
+
+[@CInline]
+let make_r2_modq r2 =
+  r2.(0ul) <- u64 0xa40611e3449c0f01;
+  r2.(1ul) <- u64 0xd00e1ba768859347;
+  r2.(2ul) <- u64 0xceec73d217f5be65;
+  r2.(3ul) <- u64 0x399411b7c309a3d;
+  assert_norm (pow2 512 % Spec.Ed25519.q ==
+    0xa40611e3449c0f01 + 0xd00e1ba768859347 * pow2 64 +
+    0xceec73d217f5be65 * pow2 128 + 0x399411b7c309a3d * pow2 192);
+  let h = ST.get () in
+  SD.bn_eval_unfold_i (as_seq h r2) 4;
+  SD.bn_eval_unfold_i (as_seq h r2) 3;
+  SD.bn_eval_unfold_i (as_seq h r2) 2;
+  SD.bn_eval_unfold_i (as_seq h r2) 1;
+  SD.bn_eval0 (as_seq h r2)
+
+
+val modq: a:lbuffer uint64 8ul -> res:lbuffer uint64 4ul ->
+  Stack unit
+  (requires fun h ->
+    live h a /\ live h res /\ disjoint a res)
+  (ensures  fun h0 _ h1 -> modifies (loc res) h0 h1 /\
+    BD.bn_v h1 res == BD.bn_v h0 a % Spec.Ed25519.q)
+
+[@CInline]
+let modq a res =
+  push_frame ();
+  let q = create 4ul (u64 0) in
+  make_q q;
+  assert_norm (Spec.Ed25519.q % 2 = 1);
+  assert_norm (pow2 252 < Spec.Ed25519.q);
+
+  let mu = make_mu () in
+  let r2 = create 4ul (u64 0) in
+  make_r2_modq r2;
+  BR.bn_mod_slow_precomp (AM.mk_runtime_almost_mont 4ul) q mu r2 a res;
+  pop_frame ()
+
+
+val mul_add_modq:
+    a:lbuffer uint64 4ul
+  -> b:lbuffer uint64 4ul
+  -> c:lbuffer uint64 4ul
+  -> res:lbuffer uint64 4ul ->
+  Stack unit
+  (requires fun h ->
+    live h a /\ live h b /\ live h c /\ live h res /\
+    eq_or_disjoint a b /\
+    disjoint res a /\ disjoint res b /\ disjoint res c /\
+    BD.bn_v h a < Spec.Ed25519.q /\ BD.bn_v h c < Spec.Ed25519.q)
+  (ensures  fun h0 _ h1 -> modifies (loc res) h0 h1 /\
+    BD.bn_v h1 res ==
+    (BD.bn_v h0 c + BD.bn_v h0 a * BD.bn_v h0 b) % Spec.Ed25519.q)
+
+[@CInline]
+let mul_add_modq a b c res =
+  push_frame ();
+  let tmp = create 8ul (u64 0) in
+  BN.bn_mul 4ul 4ul a b tmp;
+  let h0 = ST.get () in
+  SN.bn_mul_lemma (as_seq h0 a) (as_seq h0 b);
+  //assert (BD.bn_v h0 tmp == BD.bn_v h0 a * BD.bn_v h0 b);
+  SD.bn_eval_bound (as_seq h0 b) 4;
+  lemma_mul_lt (BD.bn_v h0 a) (BD.bn_v h0 b) Spec.Ed25519.q (pow2 256);
+  assert_norm (Spec.Ed25519.q + Spec.Ed25519.q * pow2 256 < pow2 512);
+
+  let c1 = BN.bn_add 8ul tmp 4ul c tmp in
+  let h1 = ST.get () in
+  SN.bn_add_lemma (as_seq h0 tmp) (as_seq h0 c);
+  assert (BD.bn_v h1 tmp + v c1 * pow2 512 == BD.bn_v h0 tmp + BD.bn_v h0 c);
+  SD.bn_eval_bound (as_seq h1 tmp) 8;
+  assert (v c1 = 0);
+  modq tmp res;
+  pop_frame ()
